lean/PathMapModel.lean
@@ -5,5 +5,6 @@ import PathMapModel.Write
 import PathMapModel.Map
 import PathMapModel.Spec
 import PathMapModel.Hash
+import PathMapModel.HashSecurity
 import PathMapModel.Fuzz
 import PathMapModel.Check
